all safety properties are proven

Contracts/Crowdfunding.v
@@ -151,6 +151,9 @@ transition Donate
 	        msg -> "already_donated">, MT)
  *)
 
+(* Definition of the protocol *)
+Variable crowd_addr : address.
+
 Notation tft := (trans_fun_type crowdState).
 Definition ok_msg := [:: (0, [:: 1])].
 Definition no_msg := [:: (0, [:: 0])].
@@ -162,13 +165,13 @@ Definition donate_fun : tft := fun id bal s m bc =>
     let nxt_block := block_num bc + 1 in
     let from := sender m in
     if get_max_block s <= nxt_block
-    then (s, Some (Msg 0 from 0 no_msg))
+    then (s, Some (Msg 0 crowd_addr from 0 no_msg))
     else if all [pred e | e.1 != from] bs
          (* new backer *)
          then let bs' := (from, val m) :: bs in
               let s'  := set_backers s bs' in
-              (s', Some (Msg 0 from 0 ok_msg))
-         else (s, Some (Msg 0 from 0 no_msg))
+              (s', Some (Msg 0 crowd_addr from 0 ok_msg))
+         else (s, Some (Msg 0 crowd_addr from 0 no_msg))
   else (s, None).
 
 Definition donate := CTrans donate_tag donate_fun.
@@ -200,9 +203,9 @@ Definition getfunds_fun : tft := fun id bal s m bc =>
     if (get_max_block s < blk)
     then if get_goal s <= bal
          then let s' := set_funded s true in
-              (s', Some (Msg bal from 0 ok_msg))
-         else (s, Some (Msg 0 from 0 no_msg))
-    else (s, Some (Msg 0 from 0 no_msg))
+              (s', Some (Msg bal crowd_addr from 0 ok_msg))
+         else (s, Some (Msg 0 crowd_addr from 0 no_msg))
+    else (s, Some (Msg 0 crowd_addr from 0 no_msg))
   else (s, None).
 
 Definition get_funds := CTrans getfunds_tag getfunds_fun.
@@ -238,17 +241,17 @@ Definition claim_fun : tft := fun id bal s m bc =>
     if blk <= get_max_block s
     then
       (* Too early! *)
-      (s, Some (Msg 0 from 0 no_msg))
+      (s, Some (Msg 0 crowd_addr from 0 no_msg))
     else let bs := backers s in
          if [|| funded s | get_goal s <= bal]
          (* Cannot reimburse: campaign suceeded *)
-         then (s, Some (Msg 0 from 0 no_msg))
+         then (s, Some (Msg 0 crowd_addr from 0 no_msg))
          else let n := seq.find [pred e | e.1 == from] bs in
               if n < size bs
               then let v := nth 0 (map snd bs) n in
                    let bs' := filter [pred e | e.1 != from] bs in
                    let s'  := set_backers s bs' in
-                   (s', Some (Msg v from 0 no_msg))
+                   (s', Some (Msg v crowd_addr from 0 ok_msg))
               else
                 (* Didn't back or already claimed *)
                 (s, None)
@@ -256,14 +259,19 @@ Definition claim_fun : tft := fun id bal s m bc =>
 
 Definition claim := CTrans claim_tag claim_fun.
 
-(* Definition of the protocol *)
-Variable crowd_addr : address.
-
 Program Definition crowd_prot : Protocol crowdState :=
   @CProt _ crowd_addr 0 init_state [:: donate; get_funds; claim] _.
 
 Lemma crowd_tags : tags crowd_prot = [:: 1; 2; 3].
 Proof. by []. Qed.
+
+Lemma find_leq {A : eqType} (p : pred (A * nat)) (bs : seq (A * nat)) :
+  nth 0 [seq i.2 | i <- bs] (seq.find p bs) <= sumn [seq i.2 | i <- bs].
+Proof.
+elim: bs=>//[[a w]]bs/=Gi; case:ifP=>_/=; first by rewrite leq_addr.
+by rewrite (leq_trans Gi (leq_addl w _)).
+Qed.
+
 
 (***********************************************************)
 (**             Correctness properties                    **)
@@ -282,6 +290,7 @@ Perhaps, we should make it stronger, adding a temporal property that
 one's reimbursement doesn't change.
 **********************************************************)
 
+   
 Definition balance_backed (st: cstate crowdState) : Prop :=
   (* If the campaign not funded... *)
   ~~ (funded (state st)) ->
@@ -321,18 +330,28 @@ case: ifP=>//=G/=; move/Hi=>/={Hi}Hi.
 rewrite addnC.
 have H1: nth 0 [seq i.2 | i <- backers s]
              (seq.find [pred e | e.1 == sender m] (backers s)) <=
-         sumn [seq i.2 | i <- backers s].
-- (* sumn_cat *)
-  by admit. (* Boring and trivial *)
+         sumn [seq i.2 | i <- backers s] by apply: find_leq.
 move: (leq_trans H1 Hi)=> H2.
 rewrite -(addnBA _ H2); clear H2.
 suff H3: sumn [seq i.2 | i <- backers s & [pred e | e.1 != sender m] i] <=
          bal - nth 0 [seq i.2 | i <- backers s]
                    (seq.find [pred e | e.1 == sender m] (backers s)).
--  by apply: (leq_trans H3 (leq_addl (val m) _ )).
-   admit.
-(* Proven modulo super-boring manipulation with sums... *)
-Admitted.
+- by apply: (leq_trans H3 (leq_addl (val m) _ )).
+clear M.
+suff H2: sumn [seq i.2 | i <- backers s & [pred e | e.1 != sender m] i] <=
+         sumn [seq i.2 | i <- backers s] -
+         nth 0 [seq i.2 | i <- backers s] (seq.find [pred e | e.1 == sender m] (backers s)).
+- by apply: (leq_trans H2); apply: leq_sub.
+clear Hi H1 X G bc bal id crowd_addr init_goal init_max_block init_owner.
+move: (backers s)=>bs{s}.
+elim:bs=>//[[a v]] bs/= Hi/=; case:ifP; last first.
+- move/negbT; case: ifP=>//= _ _; rewrite addnC -addnBA//subnn addn0.
+  clear Hi; elim: bs=>//={a v}[[a v]]bs/=.
+  case:ifP=>//=_ H; first by rewrite leq_add2l. 
+  by rewrite (leq_trans H (leq_addl _ _)).
+move/negbTE=>->/={a}; rewrite -(leq_add2l v) in Hi. 
+by rewrite addnBA in Hi; last by apply: find_leq.
+Qed.
 
 (********************************************************)
 (******   Proving temporal properties              ******)
@@ -341,9 +360,6 @@ Admitted.
 (* Contribution of backer b is d is recorded in the `backers` *)
 Definition donated b (d : value) st :=
   (filter [pred e | e.1 == b] (backers (state st))) == [:: (b, d)].
-
-Definition keeps_donation b d (st st' : cstate crowdState) :=
-  (filter [pred e | e.1 == b] (backers (state st'))) == [:: (b, d)].
 
 (* b doesn't claim its funding back *)
 Definition no_claims_from b (q : bstate * message) := sender q.2 != b.
@@ -365,7 +381,7 @@ of failure of the campaign.
 
 Lemma donation_preserved (b : address) (d : value):
   since_as_long crowd_prot (donated b d)
-                (keeps_donation b d) (no_claims_from b).
+                (fun _ s' => donated b d s') (no_claims_from b).
 Proof.
 (* This is where we would need a temporal logic, but, well.. *)
 (* Let's prove it out of the definition. *)
@@ -404,13 +420,41 @@ TODO: formulate and prove it.
 
 ************************************************************************)
 
+Lemma can_claim_back b d st bc:
+  (* We have donated, so the contract holds that state *)
+  donated b d st ->
+  (* Not funded *)
+  ~~(funded (state st)) ->
+  (* Balance is small: not reached the goal *)
+  balance st < (get_goal (state st)) ->
+  (* Block number exceeds the set number *)
+  get_max_block (state st) < block_num bc ->
+  (* Can emit message from b *)
+  exists (m : message),
+    sender m == b /\
+    out (step_prot crowd_prot st bc m) = Some (Msg d crowd_addr b 0 ok_msg).
+Proof.
+move=>D Nf Nb Nm.
+exists (Msg 0 b crowd_addr claim_tag [::]); split=>//.
+rewrite /step_prot.
+case: st D Nf Nb Nm =>id bal s/= D Nf Nb Nm.
+rewrite /apply_prot/=/claim_fun/=leqNgt Nm/= leqNgt Nb/=.
+rewrite /donated/= in D.
+move/negbTE: Nf=>->/=; rewrite -(has_find [pred e | e.1 == b]) has_filter.
+move/eqP: D=>D; rewrite D/=.
+congr (Some _); congr (Msg _ _ _ _ _). 
+elim: (backers s) D=>//[[a w]]bs/=; case:ifP; first by move/eqP=>->{a}/=_; case. 
+by move=>X Hi H; move/Hi: H=><-. 
+Qed.
+
 
 (************************************************************************
 
 4. Can we have a logic that allows to express all these properties
 declaratively? Perhaps, we could do it in TLA?
 
-************************************************************************)
+(This is going to be our future work.)
 
+************************************************************************)
 
 End Crowdfunding.
